src/Bisimulations.v
@@ -154,12 +154,12 @@ Proof.
     exists q, q'. split. auto. split; auto. apply internals_refl.
 Qed.
 
-Goal Node_equivalence ([], 
+Goal forall ether, Node_equivalence (ether, 
                          0 : inl ([], ELet "X"%string (ELit 0%Z) (EVar 0), [], [], false) ||||
                          1 : inl ([], EConcBIF (ELit "send"%string) [EPid 0;ELit 1%Z], [], [], false) ||||
                          nullpool
                       )
-                      ([],
+                      (ether,
                         0 : inl ([], ELit 0%Z, [], [], false) ||||
                         1 : inl ([], EConcBIF (ELit "send"%string) [EPid 0;ELit 1%Z], [], [], false) ||||
                         nullpool
