src/Examples.v
@@ -7,13 +7,19 @@ Import ListNotations.
   3 : 2 + 3 == 5
 *)
 Open Scope string_scope. Print LiveProcess.
+
+Ltac ether_cleanup :=
+  unfold nullpool, etherAdd;
+  repeat rewrite update_same;
+  repeat (rewrite update_noop; [|unfold nullpool;cbn;reflexivity]).
+
 Goal exists acts k,
-  ([], 0 : inl ([], EConcBIF (ELit "send") [EPid 1;EPlus (ELit 1%Z) (ELit 1%Z)], [], [], false) ||||
+  (fun _ => [], 0 : inl ([], EConcBIF (ELit "send") [EPid 1;EPlus (ELit 1%Z) (ELit 1%Z)], [], [], false) ||||
        1 : inl ([], EReceive [(PVar, EConcBIF (ELit "send") [EPid 3;EVar 0])], [], [], false) ||||
        2 : inl ([], EConcBIF (ELit "send") [EPid 3;ELit 3%Z], [], [], false) ||||
        3 : inl ([], EReceive [(PVar, EReceive [(PVar, EPlus (EVar 0) (EVar 1))])], [], [], false) |||| nullpool)
   -[ k | acts ]ₙ->*
-  ([], 0 : inl ([], ELit 2%Z, [], [], false) ||||
+  (fun _ => [], 0 : inl ([], ELit 2%Z, [], [], false) ||||
        1 : inl ([], ELit 2%Z, [], [], false) ||||
        2 : inl ([], ELit 3%Z, [], [], false) ||||
        3 : inl ([], ELit 5%Z, [], [], false) |||| nullpool).
@@ -52,9 +58,9 @@ Proof.
   simpl.
 
   rewrite par_swap with (ι' := 3). 2: lia.
-  eapply n_trans. apply n_arrive. 
-    constructor. reflexivity. repeat constructor.
-  cbn. break_match_goal. 2: congruence.
+  eapply n_trans. apply n_arrive with (ι0 := 2).
+    reflexivity. repeat constructor.
+  cbn.
 
   rewrite par_swap with (ι' := 0). rewrite par_swap with (ι' := 0). 2-3: lia.
 
@@ -66,9 +72,9 @@ Proof.
   constructor. constructor. simpl.
 
   rewrite par_swap with (ι' := 1). 2: lia.
-  eapply n_trans. apply n_arrive.
-    constructor. reflexivity. repeat constructor.
-  cbn. break_match_goal. 2: congruence.
+  eapply n_trans. apply n_arrive with (ι0 := 0).
+    reflexivity. repeat constructor.
+  cbn.
 
   (* Now with 1 *)
   eapply n_trans. eapply n_other with (ι := 1).
@@ -89,9 +95,9 @@ Proof.
 
   rewrite par_swap with (ι' := 3). 2: lia.
 
-  eapply n_trans. apply n_arrive.
-    constructor. reflexivity. repeat constructor.
-    cbn. break_match_goal. 2: congruence.
+  eapply n_trans. apply n_arrive with (ι0 := 1).
+    reflexivity. repeat constructor.
+  cbn.
 
   (* Mailbox processing for 3 *)
   eapply n_trans. eapply n_other with (ι := 3).
@@ -111,6 +117,7 @@ Proof.
   rewrite par_swap with (ι' := 0). rewrite par_swap with (ι' := 0).
   rewrite par_swap with (ι' := 1). rewrite par_swap with (ι' := 2).
 
+  ether_cleanup.
   apply n_refl.
   all: lia.
 Qed.
@@ -128,14 +135,14 @@ let X = spawn(fun() -> receive X -> X ! self() end end, [])
 
 *)
 Goal exists acts k,
-  ([], 0 : inl ([], ELet "X" (EConcBIF (ELit "spawn") [EFun [] (EReceive [(PVar, EConcBIF (ELit "send") [EVar 0; EConcBIF (ELit "self") []])]);
+  (fun _ => [], 0 : inl ([], ELet "X" (EConcBIF (ELit "spawn") [EFun [] (EReceive [(PVar, EConcBIF (ELit "send") [EVar 0; EConcBIF (ELit "self") []])]);
                                              ENil])
              (ELet "Y"%string (EConcBIF (ELit "send") [EVar 0; EConcBIF (ELit "self") []])
                  (EReceive [(PVar, EVar 0)]))
                   , [], [], false)
   |||| nullpool)
   -[ k | acts ]ₙ->*
-  ([], 0 : inl ([], EPid 1, [], [], false) ||||
+  (fun _ => [], 0 : inl ([], EPid 1, [], [], false) ||||
        1 : inl ([], EPid 1, [], [], false) |||| nullpool).
 Proof.
   eexists. exists 26.
@@ -194,9 +201,9 @@ Proof.
   simpl.
   rewrite par_swap with (ι' := 1). 2: lia.
 
-  eapply n_trans. apply n_arrive.
-    constructor. reflexivity. repeat constructor.
-  cbn. break_match_goal. 2: congruence.
+  eapply n_trans. apply n_arrive with (ι0 := 0).
+    reflexivity. repeat constructor.
+  cbn.
   eapply n_trans. eapply n_other with (ι := 1).
     apply p_receive; auto; try reflexivity. right. right. left. eexists. auto.
   simpl.
@@ -216,23 +223,23 @@ Proof.
 
   rewrite par_swap with (ι' := 0). 2: lia.
 
-  eapply n_trans. apply n_arrive.
-    constructor. reflexivity. repeat constructor.
+  eapply n_trans. apply n_arrive with (ι0 := 1).
+    reflexivity. repeat constructor.
   eapply n_trans. eapply n_other with (ι := 0).
     apply p_receive; auto. reflexivity. right. right. left. eexists. auto. cbn.
   break_match_goal. 2: congruence.
   cbn. break_match_goal. 2: congruence.
-  break_match_goal. 2: congruence.
+  ether_cleanup.
   apply n_refl.
 Qed.
 
 Goal exists k acts,
-  ([], 0 : inl ([], ELit 2%Z, [], [], false) ||||
+  (fun _ => [], 0 : inl ([], ELit 2%Z, [], [], false) ||||
        1 : inl ([], ELit 2%Z, [], [], false) ||||
        2 : inl ([], ELit 3%Z, [], [], false) ||||
        3 : inl ([], ELit 5%Z, [], [], false) |||| nullpool)
   -[k | acts]ₙ->*
-  ([], nullpool).
+  (fun _ => [], nullpool).
 Proof.
   exists 8. eexists.
   eapply n_trans. eapply n_other with (ι := 0).
@@ -267,11 +274,11 @@ Qed.
 
 (* trapping kill which comes from link *)
 Goal exists k acts,
-  ([], 0 : inl ([], ELet "X" (EConcBIF link [EPid 1])
+  (fun _ => [], 0 : inl ([], ELet "X" (EConcBIF link [EPid 1])
                              (EConcBIF exit [kill]), [], [], false) ||||
        1 : inl ([], EReceive [(PVar, EVar 0)], [], [], true) |||| nullpool)
   -[k | acts]ₙ->*
-  ([], 1 : inl ([], VCons (EXIT) (VCons (EPid 0) (VCons kill ENil)), [], [0], true)
+  (fun _ => [], 1 : inl ([], VCons (EXIT) (VCons (EPid 0) (VCons kill ENil)), [], [0], true)
            |||| nullpool).
 Proof.
   do 2 eexists.
@@ -299,27 +306,28 @@ Proof.
   simpl.
   eapply n_trans. apply n_terminate.
     rewrite update_swap. rewrite nullpool_remove. 2: lia.
-  eapply n_trans. eapply n_arrive.
+  eapply n_trans. eapply n_arrive with (ι0 := 0).
+    reflexivity.
     do 2 constructor.
-    do 2 constructor.
-  cbn. break_match_goal. 2: congruence.
-  eapply n_trans. eapply n_arrive.
+  cbn.
+  eapply n_trans. eapply n_arrive with (ι0 := 0).
     do 2 constructor.
     eapply p_exit_convert. right. split; auto. now constructor.
-  cbn. break_match_goal. 2: congruence.
+  cbn.
   eapply n_trans. eapply n_other with (ι := 1).
     apply p_receive; try reflexivity. do 2 right. left. eexists. reflexivity.
   cbn. break_match_goal. 2: congruence.
+  ether_cleanup.
   apply n_refl.
 Qed.
 
 (* kill through link, without traps -> no conversion to killed *)
 Goal exists k acts,
-  ([], 0 : inl ([], ELet "X" (EConcBIF link [EPid 1])
+  (fun _ => [], 0 : inl ([], ELet "X" (EConcBIF link [EPid 1])
                              (EConcBIF exit [kill]), [], [], false) ||||
        1 : inl ([], EReceive [(PVar, EVar 0)], [], [], false) |||| nullpool)
   -[k | acts]ₙ->*
-  ([], 1 : inr [(0, kill)]
+  (fun _ => [], 1 : inr [(0, kill)]
            |||| nullpool).
 Proof.
   do 2 eexists.
@@ -347,26 +355,27 @@ Proof.
   simpl.
   eapply n_trans. apply n_terminate.
     rewrite update_swap. rewrite nullpool_remove. 2: lia.
-  eapply n_trans. eapply n_arrive.
+  eapply n_trans. eapply n_arrive with (ι0 := 0).
+    reflexivity.
     do 2 constructor.
-    do 2 constructor.
-  cbn. break_match_goal. 2: congruence.
-  eapply n_trans. eapply n_arrive.
+  cbn.
+  eapply n_trans. eapply n_arrive with (ι0 := 0).
     do 2 constructor.
   eapply p_exit_terminate. right. left. repeat split; auto.
     1-3: intros; try congruence. now constructor.
-  cbn. break_match_goal. 2: congruence.
+  cbn.
+  ether_cleanup.
   apply n_refl.
 Qed.
 
 (* kill sent explicitly, converted to killed *)
 Goal exists k acts,
-  ([], 0 : inl ([], ELet "X" (EConcBIF link [EPid 1])
+  (fun _ => [], 0 : inl ([], ELet "X" (EConcBIF link [EPid 1])
                              (ELet "X" (EConcBIF exit [EPid 1; kill])
                                        (EReceive [(PVar, ENil)])), [], [], false) ||||
        1 : inl ([], EReceive [(PVar, EVar 0)], [], [], false) |||| nullpool)
   -[k | acts]ₙ->*
-  ([], 0 : inr [(1, killed)]
+  (fun _ => [], 0 : inr [(1, killed)]
            |||| nullpool).
 Proof.
   do 2 eexists.
@@ -397,34 +406,36 @@ Proof.
     do 3 constructor. auto.
   simpl.
   rewrite par_swap. 2: lia.
-  eapply n_trans. eapply n_arrive.
+  eapply n_trans. eapply n_arrive with (ι0 := 0).
+    reflexivity.
     do 2 constructor.
-    do 2 constructor.
-  cbn. break_match_goal. 2: congruence.
-  eapply n_trans. eapply n_arrive.
-    do 2 constructor.
+  cbn.
+  eapply n_trans. eapply n_arrive with (ι0 := 0).
+    reflexivity.
     apply p_exit_terminate. auto.
-  cbn. break_match_goal. 2: congruence.
+  cbn.
   eapply n_trans. apply n_send.
     apply p_dead. simpl.
   eapply n_trans. apply n_terminate.
-    rewrite update_swap, nullpool_remove. 2: lia.
-  eapply n_trans. eapply n_arrive.
-    do 2 constructor.
+    ether_cleanup.
+    rewrite update_swap with (p := None). rewrite nullpool_remove. 2: lia.
+  eapply n_trans. eapply n_arrive with (ι0 := 1).
+    reflexivity.
     apply p_exit_terminate.
     right. left. intuition; auto. congruence.
-  cbn. break_match_goal. 2: congruence.
+  cbn.
+  ether_cleanup.
   apply n_refl.
 Qed.
 
 (* trapping exits *)
 Goal exists k acts,
-  ([], 0 : inl ([], EReceive [(PVar, EConcBIF exit [EPid 1; ELit "foo"])], [], [], false) ||||
+  (fun _ => [], 0 : inl ([], EReceive [(PVar, EConcBIF exit [EPid 1; ELit "foo"])], [], [], false) ||||
        1 : inl ([], ELet "X" (ELet "X" (EConcBIF process_flag [trap_exit; tt]) 
                                        (EConcBIF send [EPid 0; ENil])) 
                              (EReceive [(PVar, EVar 0)]), [], [], false) |||| nullpool)
   -[k | acts]ₙ->*
-  ([], 1 : inl ([], VCons EXIT (VCons (EPid 0) (VCons (ELit "foo") ENil)), [], [], true)
+  (fun _ => [], 1 : inl ([], VCons EXIT (VCons (EPid 0) (VCons (ELit "foo") ENil)), [], [], true)
            |||| nullpool).
 Proof.
   do 2 eexists.
@@ -455,10 +466,10 @@ Proof.
   eapply n_trans. eapply n_other with (ι := 1).
     do 3 constructor. auto. simpl.
   rewrite par_swap. 2: lia.
-  eapply n_trans. eapply n_arrive.
+  eapply n_trans. eapply n_arrive with (ι0 := 1).
+    reflexivity.
     do 2 constructor.
-    do 2 constructor.
-  cbn. break_match_goal. 2: congruence.
+  cbn.
   eapply n_trans. eapply n_other.
     apply p_receive. 1-2: reflexivity. do 2 right. left. now eexists.
   cbn. break_match_goal. 2: congruence.
@@ -474,23 +485,24 @@ Proof.
     apply p_terminate. constructor. auto.
   eapply n_trans. apply n_terminate.
   rewrite update_swap, nullpool_remove. 2: lia.
-  eapply n_trans. apply n_arrive.
-    do 2 constructor.
+  eapply n_trans. apply n_arrive with (ι0 := 0).
+    reflexivity.
     apply p_exit_convert. left. split; auto. congruence.
-  cbn. break_match_goal. 2: congruence.
+  cbn.
   eapply n_trans. apply n_other.
     apply p_receive. 1-2: reflexivity. do 2 right; left; now eexists.
   cbn. break_match_goal. 2: congruence.
+  ether_cleanup.
   apply n_refl.
 Qed.
 
 (* explicit exit signal drop *)
 Goal exists k acts,
-  ([], 0 : inl ([], ELet "X" (EConcBIF exit [EPid 1; ELit "normal"]) 
+  (fun _ => [], 0 : inl ([], ELet "X" (EConcBIF exit [EPid 1; ELit "normal"]) 
                              (EConcBIF send [EPid 1; ENil]), [], [], false) ||||
        1 : inl ([], EReceive [(PVar, EVar 0)], [], [], false) |||| nullpool)
   -[k | acts]ₙ->*
-  ([], 0 : inl ([], ENil, [], [], false) ||||
+  (fun _ => [], 0 : inl ([], ENil, [], [], false) ||||
        1 : inl ([], ENil, [], [], false) |||| nullpool).
 Proof.
   do 2 eexists.
@@ -515,27 +527,28 @@ Proof.
   eapply n_trans. eapply n_send with (ι := 0).
     do 3 constructor. simpl.
   rewrite par_swap. 2: lia.
-  eapply n_trans. apply n_arrive.
+  eapply n_trans. apply n_arrive with (ι0 := 0).
     do 2 constructor.
     apply p_exit_drop. left. auto.
-  cbn. break_match_goal. 2: congruence.
-  eapply n_trans. apply n_arrive.
+  cbn.
+  eapply n_trans. apply n_arrive with (ι0 := 0).
     do 2 constructor.
     apply p_arrive; constructor.
-  cbn. break_match_goal. 2: congruence.
+  cbn.
   eapply n_trans. apply n_other.
     apply p_receive. 1-2: reflexivity. do 2 right; left; now eexists.
   cbn. break_match_goal. 2: congruence.
   rewrite par_swap. 2: lia.
+  ether_cleanup.
   apply n_refl.
 Qed.
 
 (* implicit exit signal drop *)
 Goal exists k acts,
-  ([], 0 : inl ([], ELet "X" (ELit 1%Z) (EVar 0), [], [], false) ||||
+  (fun _ => [], 0 : inl ([], ELet "X" (ELit 1%Z) (EVar 0), [], [], false) ||||
        1 : inl ([], EReceive [(PVar, EVar 0)], [], [], false) |||| nullpool)
   -[k | acts]ₙ->*
-  ([], 1 : inl ([], EReceive [(PVar, EVar 0)], [], [], false) |||| nullpool).
+  (fun _ => [], 1 : inl ([], EReceive [(PVar, EVar 0)], [], [], false) |||| nullpool).
 Proof.
   do 2 eexists.
   eapply n_trans. eapply n_other.
